mam/Cislo6.lean
@@ -1,37 +1,41 @@
-import Mathlib.Tactic.Linarith
+import mam.Reseni5
 
 
-def ciferny_soucet (a : Nat) : Nat :=
+def ciferny_soucet' (a : Nat) : Nat :=
 if a < 10
 then a
-else (a % 10) + ciferny_soucet (a / 10)
+else (a % 10) + ciferny_soucet' (a / 10)
 decreasing_by
   simp_wf
-  have : a ≥ 10
-  · apply le_of_not_lt
-    assumption
-  have : a / 10 ≥ 10 / 10
-  · exact Nat.div_le_div_right this
-  have : a / 10 ≥ 1
-  · convert this
-  have : a / 10 < a / 10 * 10
-  · linarith
   have : a / 10 * 10 ≤ a
   · exact Nat.div_mul_le_self a 10
   linarith
 
-#eval ciferny_soucet 524
-#eval ciferny_soucet 10200
-#eval ciferny_soucet (10^50 - 1)
-#eval ciferny_soucet 0
+#eval ciferny_soucet' 524
+#eval ciferny_soucet' 10200
+#eval ciferny_soucet' (10^50 - 1)
+#eval ciferny_soucet' 0
 
 
-def ackermann : Nat → Nat → Nat
+def ackermann' : Nat → Nat → Nat
 | 0  , n   => n+1
-| m+1, 0   => ackermann m 1
-| m+1, n+1 => ackermann m (ackermann (m+1) n)
-termination_by ackermann m n => (m, n)
+| m+1, 0   => ackermann' m 1
+| m+1, n+1 => ackermann' m (ackermann' (m+1) n)
+termination_by
+  ackermann' m n => (m, n)
 
-#eval ackermann 2 100
-#eval ackermann 3 0
-#eval ackermann 3 5
+#eval ackermann' 2 100
+#eval ackermann' 3 0
+#eval ackermann' 3 5
+
+
+lemma obrat_rychl_vs_obrat {T : Type} (x y : List T) : obrat_rychl x y = obrat y ++ x := by
+  induction y generalizing x with
+  | nil => simp [obrat_rychl, obrat]
+  | cons d l ih => simp [obrat_rychl, obrat, ih]
+
+theorem obrat_rychle_vs_obrat {T : Type} : @obrat_rychle T = @obrat T := by
+  simp [obrat_rychle, obrat_rychl_vs_obrat]
+
+theorem obrat_rychle_obrat_rychle {T : Type} (l : List T) : obrat_rychle (obrat_rychle l) = l := by
+  rw [obrat_rychle_vs_obrat, obrat_obrat]
