mam/Reseni5.lean
@@ -1,0 +1,43 @@
+import mam.Cislo5
+
+
+def prvnich_n_krychli_sestupne : ℕ → List ℕ
+| 0   => []
+| n+1 => n^3 :: prvnich_n_krychli_sestupne n
+
+def prvnich_n_krychli : ℕ → List ℕ :=
+obrat ∘ prvnich_n_krychli_sestupne
+
+lemma soucet_prvnich_n_krychli_sestupne (m : ℕ) :
+    soucet (prvnich_n_krychli_sestupne m.succ) * 4 = (m ^ 2 * m.succ ^ 2) := by
+  induction m with
+  | zero => decide
+  | succ n ih =>
+    convert_to ((n+1) ^ 3 + soucet (prvnich_n_krychli_sestupne (n+1))) * 4 = (n+1) ^ 2 * (n+2) ^ 2
+    convert_to (n+1) ^ 3 * 4 + soucet (prvnich_n_krychli_sestupne (n+1)) * 4 = (n+1) ^ 2 * (n+2) ^ 2
+    · ring
+    rw [ih]
+    convert_to (n+1) ^ 3 * 4 + n ^ 2 * (n+1) ^ 2 = (n+1) ^ 2 * (n+2) ^ 2
+    ring
+
+theorem soucet_prvnich_n_krychli (n : ℕ) :
+    soucet (prvnich_n_krychli n) = ((n-1) ^ 2 * n ^ 2) / 4 := by
+  cases n with
+  | zero => decide
+  | succ m =>
+    dsimp [prvnich_n_krychli]
+    rw [obrat_zachovava_soucet]
+    convert_to soucet (prvnich_n_krychli_sestupne m.succ) = m^2 * m.succ^2 / 4
+    rw [←soucet_prvnich_n_krychli_sestupne m]
+    simp
+
+
+lemma obrat_pripoj {T : Type} (x : List T) (a : T) : obrat (x ++ [a]) = a :: obrat x := by
+  induction x with
+  | nil => rfl
+  | cons d l ih => simp [obrat, ih]
+
+theorem obrat_obrat {T : Type} (x : List T) : obrat (obrat x) = x := by
+  induction x with
+  | nil => rfl
+  | cons d l ih => simp [obrat, ih, obrat_pripoj]
